Finished the definition of client model

fairness/examples/ticketlock/client_model.v
@@ -155,24 +155,24 @@ Section ClientDefs.
 
   (* TODO: reorganize the premises so those below don't depend
      on the client's choice of lib_gs *)
-  Let tl_st := fmstate TlLM_FM. 
+  Let tl_state := fmstate TlLM_FM. 
   Let tl_role := fmrole TlLM_FM.
   Let tl_erole := @ext_role _ TlEM.
 
   Context
-    {allows_unlock: tl_st → tl_st → Prop}
-    {allows_lock: tl_role → tl_st → tl_st → Prop}
-    {tl_active_exts: tl_st → gset (fl_EI (M := TlLM_FM))}
+    {allows_unlock: tl_state → tl_state → Prop}
+    {allows_lock: tl_role → tl_state → tl_state → Prop}
+    {tl_active_exts: tl_state → gset (fl_EI (M := TlLM_FM))}
     (tl_active_exts_spec: ∀ st ι,
         ι ∈ tl_active_exts st ↔ (∃ st', @fl_ETs _ allows_unlock allows_lock ι st st')). 
-  Context {can_lock_st has_lock_st active_st: tl_role → tl_st → Prop}. 
-  Context {is_init_st: tl_st → Prop}.
+  Context {can_lock_st has_lock_st active_st: tl_role → tl_state → Prop}. 
+  Context {is_init_st: tl_state → Prop}.
 
   Context (TlEM_FL: @FairLock TlLM_FM _ _ _ tl_active_exts_spec
                       can_lock_st has_lock_st active_st is_init_st).
 
   Inductive flag_state := | fs_U | fs_S | fs_O. 
-  Definition client_state: Type := tl_st * flag_state.
+  Definition client_state: Type := tl_state * flag_state.
 
   (* Inductive cl_role := | cl_l | cl_r.  *)
   Inductive cl_role_kind := | cl_lift | cl_au | cl_al | cl_cl.
@@ -197,9 +197,9 @@ Section ClientDefs.
       (LOCK: has_lock_st ρlg tl)
       (DIS: ¬ active_st ρlg tl):
     client_trans (tl, fs_S) (Some (cl_au, cl_L)) (allow_unlock_impl tl, fs_S)
-  | ct_au_R tl fs
+  | ct_au_R tl fs fs'
       (ρlg := ρlg_r)
-      (fs' := match fs with | fs_U => fs_U | _ => fs_O end) (* fs=O is impossible though*)
+      (FS: fs = fs_U /\ fs' = fs_U \/ fs = fs_S /\ fs' = fs_O)
       (LOCK: has_lock_st ρlg tl)
       (DIS: ¬ active_st ρlg tl):
     client_trans (tl, fs) (Some (cl_au, cl_R)) (allow_unlock_impl tl, fs')
@@ -209,6 +209,112 @@ Section ClientDefs.
       (DIS: ¬ active_st ρlg tl)
       (NO: fs ≠ fs_O):
     client_trans (tl, fs) (Some (cl_al, cl_R)) (allow_lock_impl ρlg tl, fs)
-  . 
+  .
+
+  Instance cl_role_kind_dec: EqDecision cl_role_kind.
+  Proof. solve_decision. Qed. 
+  Instance flag_state_dec: EqDecision flag_state.
+  Proof. solve_decision. Qed.   
+  Instance cl_id_dec: EqDecision cl_id.
+  Proof. solve_decision. Qed.
+
+  Ltac fin_type_countable all_values :=
+    unshelve eapply finite.finite_countable;
+    refine {| finite.enum := all_values |};
+    [ repeat (apply NoDup_cons; split; [set_solver| ]); apply NoDup_nil_2 |
+     by intros x; destruct x; set_solver]. 
+       
+  Instance cl_role_kind_cnt: Countable cl_role_kind.
+  Proof. fin_type_countable [cl_lift; cl_au; cl_al; cl_cl]. Qed. 
+  Instance flag_state_cnt: Countable flag_state.
+  Proof. fin_type_countable [fs_U; fs_S; fs_O]. Qed. 
+  Instance cl_id_cnt: Countable cl_id.
+  Proof. fin_type_countable [cl_L; cl_R]. Qed. 
+  
+  (* Lemma client_role_Cnt: Countable client_role. *)
+    
+  (*   unshelve eapply prod_countable; try apply _.   *)
+  
+  Instance client_step_ex_dec (st: client_state) (ρ: client_role):
+    Decision (exists st', client_trans st (Some ρ) st').
+  Proof.
+    destruct st as [tl_st flag].
+    destruct ρ as [k c].
+    destruct k.
+    - pose proof TlLM_LFP. (* why it's not inferred? *)
+      destruct (decide (exists tl_st', locale_trans tl_st (ρlg_tl c) tl_st' (LM := TlLM))) as [STEP | NOSTEP]. 
+      + left. destruct STEP as [? STEP].
+        eexists (_, _). eapply ct_lib_step. apply STEP.
+      + right. intros [? STEP]. inversion STEP. subst.
+        eapply NOSTEP. eexists. apply LIB_STEP.
+    - destruct c.
+      + destruct (decide (has_lock_st (ρlg_tl cl_L) tl_st /\ ¬ active_st (ρlg_tl cl_L) tl_st /\ flag = fs_S)) as [(?&?&->)| ]. 
+        * left. eexists (_, _). eapply ct_au_L; eauto.
+        * right. intros [? STEP]. inversion STEP. subst. tauto.
+      + destruct (decide (has_lock_st (ρlg_tl cl_R) tl_st /\ ¬ active_st (ρlg_tl cl_R) tl_st /\ flag ≠ fs_O)) as [(?&?&?)| ].
+        * left. eexists (_, if decide (flag = fs_U) then fs_U else fs_O). eapply ct_au_R; eauto.
+          destruct flag;
+            (rewrite decide_True; tauto) || (rewrite decide_False; try tauto; congruence).
+        * right. intros [? STEP]. inversion STEP; subst.
+          apply n. 
+          destruct FS as [[-> ->] | [-> ->]]; try tauto.
+          all: split; eauto.
+    - destruct (decide (can_lock_st (ρlg_tl cl_R) tl_st /\ ¬ active_st (ρlg_tl cl_R) tl_st /\ flag ≠ fs_O /\ c = cl_R)) as [(?&?&?&->) | NOSTEP].
+      + left. eexists (_, _). econstructor; eauto.
+      + right. intros [? STEP]. inversion STEP; subst. tauto.
+    - destruct (decide (has_lock_st (ρlg_tl cl_L) tl_st /\ ¬ active_st (ρlg_tl cl_L) tl_st /\ flag = fs_U /\ c = cl_L)) as [(?&?&->&->)| ].
+      + left. eexists (_, _). econstructor; eauto.
+      + right. intros [? STEP]. inversion STEP; subst. tauto.
+  Qed.
+
+  Definition client_lr (st: client_state): gset (client_role) :=
+    filter (fun r => (@bool_decide _ (client_step_ex_dec st r) = true))
+           (list_to_set $
+              k ← [cl_lift; cl_au; cl_al; cl_cl];
+              c ← [cl_L; cl_R];
+              mret (k, c)). 
+
+  Lemma client_lr_spec: ∀ (s : client_state) (ρ : client_role),
+      (exists s', client_trans s (Some ρ) s') <-> ρ ∈ client_lr s.
+  Proof.
+    intros ??. rewrite /client_lr.
+    rewrite elem_of_filter. rewrite @bool_decide_eq_true.
+    rewrite iff_and_impl_helper; [done| ]. 
+    intros _. destruct ρ as [[] []]; set_solver.  
+  Qed. 
+
+    
+  Definition client_model_impl: FairModel.
+  Proof.
+    refine ({|
+        fmstate := client_state; 
+        fmrole := client_role;
+        fmtrans := client_trans;
+        live_roles := client_lr;
+    |}).
+    - pose proof (@LS_eqdec _ _ _ _ _ _ TlLM_LFP). (* not inferred? *)
+      solve_decision.
+    - pose proof (@inhLM _ _ _ _ _ _ TlLM_LFP) as [δ]. 
+      apply (populate (δ, fs_U)).
+    - apply (populate (cl_cl, cl_L)).
+    - intros. apply client_lr_spec. eauto.
+  Defined.  
 
 End ClientDefs. 
+
+
+Section ClientTraceTermination.
+
+  Lemma client_model_fair_term (tr: mtrace client_model
+    (* lmtr *)
+    (* (OUTER_CORR: outer_LM_trace_exposing lmtr tr) *)
+    :
+    mtrace_fairly_terminating tr.
+  Proof.
+    intros. red. intros VALID FAIR.
+    (* destruct (infinite_or_finite tr) as [INF|]; [| done]. *)
+    pose proof (trace_has_len tr) as [len LEN]. 
+
+
+
+End ClientTraceTermination.
